src/SDK/AwsEncryptionSdk.dfy
@@ -9,7 +9,19 @@ include "../StandardLibrary/UInt.dfy"
 include "../Generated/AwsCryptographicMaterialProviders.dfy"
 include "../Generated/AwsEncryptionSdk.dfy"
 include "../Util/UTF8.dfy"
+include "../AwsCryptographicMaterialProviders/Client.dfy"
+include "../Crypto/Random.dfy"
+include "../Crypto/AESEncryption.dfy"
 include "EncryptDecrypt.dfy"
+include "ConfigDefaults.dfy"
+
+include "Serialize/SerializableTypes.dfy"
+include "Serialize/Header.dfy"
+include "Serialize/HeaderTypes.dfy"
+include "Serialize/V1HeaderBody.dfy"
+include "Serialize/HeaderAuth.dfy"
+include "Serialize/SerializeFunctions.dfy"
+include "Serialize/EncryptionContext.dfy"
 
 module {:extern "Dafny.Aws.Esdk.AwsEncryptionSdkClient"} AwsEncryptionSdk {
   import opened Wrappers
@@ -18,28 +30,313 @@ module {:extern "Dafny.Aws.Esdk.AwsEncryptionSdkClient"} AwsEncryptionSdk {
   import UTF8
   import Aws.Crypto
   import Aws.Esdk
-  import EncryptDecrypt
+  import EncryptDecryptHelpers
+  import SerializableTypes
+  import Random
+  import MaterialProviders.Client
+  import AESEncryption
+  import EncryptionContext
+  import SerializeFunctions
+  import MessageBody
+  import Signature
+  import ConfigDefaults
+
+  import Header
+  import HeaderTypes
+  import HeaderAuth
+  import V1HeaderBody
 
   class AwsEncryptionSdkClient extends Esdk.IAwsEncryptionSdkClient {
         const config: Esdk.AwsEncryptionSdkClientConfig;
 
+        const commitmentPolicy: Crypto.CommitmentPolicy;
+
         constructor (config: Esdk.AwsEncryptionSdkClientConfig)
             ensures this.config == config
+
+            ensures config.commitmentPolicy.None? ==>
+              && var policy := ConfigDefaults.GetDefaultCommitmentPolicy(config.configDefaults);
+              && this.commitmentPolicy == policy
+
+            ensures config.commitmentPolicy.Some? ==>
+                this.commitmentPolicy == config.commitmentPolicy.value
         {
             this.config := config;
+            if config.commitmentPolicy.None? {
+                var defaultPolicy := ConfigDefaults.GetDefaultCommitmentPolicy(config.configDefaults);
+                this.commitmentPolicy := defaultPolicy;
+            } else {
+                this.commitmentPolicy := config.commitmentPolicy.value;
+            }
         }
 
         method Encrypt(input: Esdk.EncryptInput) returns (res: Result<Esdk.EncryptOutput, string>)
         {
-            var encryptRequest := EncryptDecrypt.EncryptRequest.WithCMM(input.plaintext, input.materialsManager).SetEncryptionContext(input.encryptionContext);
-            var e :- expect EncryptDecrypt.Encrypt(encryptRequest);
-            return Success(Esdk.EncryptOutput(ciphertext:=e));
+            // Validate encrypt request
+            // TODO: bring back once we can have Option<Trait>
+            //:- Need(request.cmm != null || request.keyring != null, "EncryptRequest.cmm OR EncryptRequest.keyring must be set.");
+            //:- Need(!(request.cmm != null && request.keyring != null), "EncryptRequest.keyring AND EncryptRequest.cmm must not both be set.");
+            var frameLength : int64 := EncryptDecryptHelpers.DEFAULT_FRAME_LENGTH;
+            if input.frameLength.Some? {
+                // TODO: uncomment this once we figure out why C# is passing 0 as the default value for these nullable
+                // fields
+                //frameLength := request.frameLength.value;
+            }
+            :- Need(frameLength > 0, "Requested frame length must be > 0");
+
+            var maxPlaintextLength := INT64_MAX_LIMIT - 1;
+            if input.maxPlaintextLength.Some? {
+                // TODO: uncomment this once we figure out why C# is passing 0 as the default value for these nullable
+                // fields
+                //maxPlaintextLength := request.maxPlaintextLength.value;
+            }
+            :- Need(maxPlaintextLength < INT64_MAX_LIMIT, "Input plaintext size too large.");
+
+
+            var cmm := input.materialsManager;
+            // TODO: bring back once we can have Option<Trait>
+            /*
+            if request.keyring == null {
+                cmm := request.cmm;
+            } else {
+                var client := new Client.AwsCryptographicMaterialProvidersClient();
+                cmm := client
+                    .CreateDefaultCryptographicMaterialsManager(Crypto.CreateDefaultCryptographicMaterialsManagerInput(
+                    keyring := request.keyring
+                ));
+            }*/
+
+            var algorithmSuiteID := input.algorithmSuiteId;
+
+            var encMatRequest := Crypto.GetEncryptionMaterialsInput(
+                encryptionContext:=input.encryptionContext,
+                commitmentPolicy:=this.commitmentPolicy,
+                algorithmSuiteId:=algorithmSuiteID,
+                maxPlaintextLength:=Option.Some(maxPlaintextLength as int64)
+            );
+
+            var output :- cmm.GetEncryptionMaterials(encMatRequest);
+
+            var encMat := output.encryptionMaterials;
+
+            // Validate encryption materials
+            :- Need(
+                Client.Materials.EncryptionMaterialsWithPlaintextDataKey(encMat),
+                "CMM returned invalid EncryptionMaterials"
+            );
+            :- Need(
+                SerializableTypes.IsESDKEncryptionContext(encMat.encryptionContext),
+                "CMM failed to return serializable encryption materials."
+            );
+            :- Need(HasUint16Len(encMat.encryptedDataKeys), "CMM returned EDKs that exceed the allowed maximum.");
+            :- Need(forall edk | edk in encMat.encryptedDataKeys
+                :: SerializableTypes.IsESDKEncryptedDataKey(edk),
+                "CMM returned non-serializable encrypted data key.");
+
+            var encryptedDataKeys: SerializableTypes.ESDKEncryptedDataKeys := encMat.encryptedDataKeys;
+
+            var esdkId := SerializableTypes.GetESDKAlgorithmSuiteId(encMat.algorithmSuiteId);
+            var suite := Client.SpecificationClient().GetSuite(encMat.algorithmSuiteId);
+            var messageID: HeaderTypes.MessageID :- Random.GenerateBytes(HeaderTypes.MESSAGE_ID_LEN as int32);
+            var derivedDataKey := EncryptDecryptHelpers.DeriveKey(encMat.plaintextDataKey.value, suite, messageID);
+
+            var canonicalEncryptionContext := EncryptionContext.GetCanonicalEncryptionContext(encMat.encryptionContext);
+
+            // Until the commitment policy has been plumbed through
+            // we can not assert assert Header.HeaderVersionSupportsCommitment?(suite, body);
+            // without the following:
+            :- Need(!suite.commitment.HKDF?, "Commitment not yet supported");
+
+            var body := HeaderTypes.HeaderBody.V1HeaderBody(
+                messageType := HeaderTypes.MessageType.TYPE_CUSTOMER_AED,
+                esdkSuiteId := esdkId,
+                messageId := messageID,
+                encryptionContext := canonicalEncryptionContext,
+                encryptedDataKeys := encryptedDataKeys,
+                contentType := HeaderTypes.ContentType.Framed,
+                headerIvLength := suite.encrypt.ivLength as nat,
+                frameLength := frameLength as uint32
+            );
+
+            var rawHeader := Header.WriteHeaderBody(body);
+
+            var iv: seq<uint8> := seq(suite.encrypt.ivLength as int, _ => 0);
+            var encryptionOutput :- AESEncryption.AESEncrypt(suite.encrypt, iv, derivedDataKey, [], rawHeader);
+                var headerAuth := HeaderTypes.HeaderAuth.AESMac(
+                headerIv := iv,
+                headerAuthTag := encryptionOutput.authTag
+            );
+
+            var header := Header.HeaderInfo(
+                body := body,
+                rawHeader := rawHeader,
+                encryptionContext := encMat.encryptionContext,
+                suite := suite,
+                headerAuth := headerAuth
+            );
+
+            // Add headerAuth requirements to Header type
+            assert Header.CorrectlyReadHeaderBody(
+                SerializeFunctions.ReadableBuffer(rawHeader, 0),
+                Success(
+                    SerializeFunctions.SuccessfulRead(
+                        body,
+                        SerializeFunctions.ReadableBuffer(rawHeader, |rawHeader|)
+                    )
+                )
+            );
+            assert Header.HeaderAuth?(suite, headerAuth);
+            assert Header.IsHeader(header);
+
+            // Encrypt the given plaintext into the framed message
+            var framedMessage :- MessageBody.EncryptMessageBody(
+                input.plaintext,
+                header,
+                derivedDataKey
+            );
+
+            if framedMessage.finalFrame.header.suite.signature.ECDSA? {
+                var msg := EncryptDecryptHelpers.SerializeMessageWithoutSignature(framedMessage);
+                var ecdsaParams := framedMessage.finalFrame.header.suite.signature.curve;
+                // TODO: This should just work, but Proof is difficult
+                :- Need(encMat.signingKey.Some?, "Missing signing key.");
+
+                var bytes :- Signature.Sign(ecdsaParams, encMat.signingKey.value, msg);
+                :- Need(|bytes| == ecdsaParams.SignatureLength() as int, "Malformed response from Sign().");
+
+                var signature := UInt16ToSeq(|bytes| as uint16) + bytes;
+                msg := msg + signature;
+                // TODO: Come back and prove this
+                // assert msg == SerializeMessageWithSignature(framedMessage, signature); // Header, frames and signature can be serialized into the stream
+            return Success(Esdk.EncryptOutput(ciphertext := msg));
+            } else {
+                var msg := EncryptDecryptHelpers.SerializeMessageWithoutSignature(framedMessage);
+                return Success(Esdk.EncryptOutput(ciphertext := msg));
+            }
         }
+
         method Decrypt(input: Esdk.DecryptInput) returns (res: Result<Esdk.DecryptOutput, string>)
         {
-            var decryptRequest := EncryptDecrypt.DecryptRequest.WithCMM(input.ciphertext, input.materialsManager);
-            var d :- expect EncryptDecrypt.Decrypt(decryptRequest);
-            return Success(Esdk.DecryptOutput(plaintext:=d));
+            // Validate decrypt request
+            // TODO: bring back once we can have Option<Trait>
+            //:- Need(request.cmm == null || request.keyring == null, "DecryptRequest.keyring OR DecryptRequest.cmm must be set (not both).");
+            //:- Need(request.cmm != null || request.keyring != null, "DecryptRequest.cmm and DecryptRequest.keyring cannot both be null.");
+
+            var cmm := input.materialsManager;
+            // TODO: bring back once we can have Option<Trait>
+            /*
+            if request.keyring == null {
+                cmm := request.cmm;
+            } else {
+                var client := new Client.AwsCryptographicMaterialProvidersClient();
+                cmm := client
+                    .CreateDefaultCryptographicMaterialsManager(Crypto.CreateDefaultCryptographicMaterialsManagerInput(
+                    keyring := request.keyring
+                ));
+            }*/
+
+            var buffer := SerializeFunctions.ReadableBuffer(input.ciphertext, 0);
+            var headerBody :- Header
+                .ReadHeaderBody(buffer)
+                .MapFailure(EncryptDecryptHelpers.MapSerializeFailure(": ReadHeaderBody"));
+
+            var rawHeader := headerBody.tail.bytes[buffer.start..headerBody.tail.start];
+
+            var esdkEncryptionContext := EncryptionContext.GetEncryptionContext(headerBody.data.encryptionContext);
+
+            var decMatRequest := Crypto.DecryptMaterialsInput(
+            algorithmSuiteId:=SerializableTypes.GetAlgorithmSuiteId(headerBody.data.esdkSuiteId),
+            commitmentPolicy:=this.commitmentPolicy,
+            encryptedDataKeys:=headerBody.data.encryptedDataKeys,
+            encryptionContext:=esdkEncryptionContext);
+            var output :- cmm.DecryptMaterials(decMatRequest);
+            var decMat := output.decryptionMaterials;
+
+            // Validate decryption materials
+            :- Need(Client.Materials.DecryptionMaterialsWithPlaintextDataKey(decMat), "CMM returned invalid DecryptMaterials");
+
+            var suite := Client
+                .SpecificationClient()
+                .GetSuite(decMat.algorithmSuiteId);
+
+            var headerAuth :- HeaderAuth
+                .ReadAESMac(headerBody.tail, suite)
+                .MapFailure(EncryptDecryptHelpers.MapSerializeFailure(": ReadAESMac"));
+
+            var decryptionKey := EncryptDecryptHelpers.DeriveKey(decMat.plaintextDataKey.value, suite, headerBody.data.messageId);
+
+            // There is nothing to compare since there was nothing to decrypt.
+            // Success means that the tag is correct.
+            var _ :- AESEncryption.AESDecrypt(
+                suite.encrypt,
+                decryptionKey,
+                [], // The header auth is for integrity, not confidentiality
+                headerAuth.data.headerAuthTag,
+                headerAuth.data.headerIv,
+                rawHeader
+            );
+
+            // TODO: add support for non-framed content
+            :- Need(headerBody.data.contentType.Framed?, "Fix me");
+
+            assert {:split_here} true;
+            // Currently the Encryption Context in the header MUST be the same
+            // as the canonical encryption context in the header body.
+            // Ideally, only the canonical encryption context needs to be serializable.
+            :- Need(SerializableTypes.IsESDKEncryptionContext(decMat.encryptionContext), "CMM failed to return serializable encryption materials.");
+            // The V2 message format not only supports commitment, it requires it.
+            // Therefore the message format is bound to properties of the algorithm suite.
+            :- Need(Header.HeaderVersionSupportsCommitment?(suite, headerBody.data), "Algorithm suite does not match message format.");
+
+            var header := Header.HeaderInfo(
+                body := headerBody.data,
+                rawHeader := rawHeader,
+                encryptionContext := decMat.encryptionContext,
+                suite := suite,
+                headerAuth := headerAuth.data
+            );
+
+            assert {:split_here} true;
+            assert Header.CorrectlyReadHeaderBody(
+            SerializeFunctions.ReadableBuffer(rawHeader, 0),
+            Success(
+                SerializeFunctions.SuccessfulRead(
+                    headerBody.data, SerializeFunctions.ReadableBuffer(rawHeader, |rawHeader|))
+                )
+            );
+            assert Header.HeaderAuth?(suite, headerAuth.data);
+            assert Header.IsHeader(header);
+
+            var messageBody :- MessageBody.ReadFramedMessageBody(
+                headerAuth.tail,
+                header,
+                [],
+                headerAuth.tail
+            ).MapFailure(EncryptDecryptHelpers.MapSerializeFailure(": ReadFramedMessageBody"));
+
+            assert {:split_here} true;
+            assert suite == messageBody.data.finalFrame.header.suite;
+            assert |decryptionKey| == messageBody.data.finalFrame.header.suite.encrypt.keyLength as int;
+
+            // ghost var endHeaderPos := rd.reader.pos;
+            // Parse the message body
+            var plaintext;
+            match header.body.contentType {
+            case NonFramed => return Failure("not at this time");
+            //   plaintext :- MessageBody.DecryptNonFramedMessageBody(rd, suite, decryptionKey, header.body.messageID);
+            case Framed =>
+                plaintext :- MessageBody.DecryptFramedMessageBody(messageBody.data, decryptionKey);
+            }
+
+            var signature :- EncryptDecryptHelpers.VerifySignature(
+                messageBody.tail,
+                messageBody.tail.bytes[buffer.start..messageBody.tail.start],
+                decMat
+            );
+
+            :- Need(signature.start == |signature.bytes|, "Data after message footer.");
+
+            return Success(Esdk.DecryptOutput(plaintext := plaintext));
         }
-  }
+    }
 }
