src/SDK/ConfigDefaults.dfy
@@ -1,0 +1,23 @@
+
+include "../Generated/AwsEncryptionSdk.dfy"
+include "../Generated/AwsCryptographicMaterialProviders.dfy"
+
+/*
+ * This module contains methods for translating the ConfigurationDefaults
+ * parameter (that is passed into client creation) into the individual
+ * default configurations it controls (e.g. commitment policy)
+ */
+module {:extern "ConfigDefaults"} ConfigDefaults {
+
+  import Aws
+
+  function method GetDefaultCommitmentPolicy(configDefaults : Aws.Esdk.ConfigurationDefaults):
+    (res: Aws.Crypto.CommitmentPolicy)
+
+    ensures
+      configDefaults == Aws.Esdk.V1 ==> res == Aws.Crypto.REQUIRE_ENCRYPT_REQUIRE_DECRYPT
+    {
+      // TODO: actual matching on version
+      Aws.Crypto.REQUIRE_ENCRYPT_REQUIRE_DECRYPT
+    }
+}
