test/SDK/POCEncryptDecrypt.dfy
@@ -45,7 +45,9 @@ module {:extern "TestClient"} TestClient {
 
     // Create AWS Crypto client
     // TODO use createClient
-    var config := Esdk.AwsEncryptionSdkClientConfig(configDefaults := Esdk.V1);
+    var config := Esdk.AwsEncryptionSdkClientConfig(
+      configDefaults := Esdk.V1, commitmentPolicy := Option.Some(Crypto.REQUIRE_ENCRYPT_REQUIRE_DECRYPT)
+    );
     var client := new AwsEncryptionSdk.AwsEncryptionSdkClient(config);
 
     // Use Encrypt API
@@ -55,7 +57,9 @@ module {:extern "TestClient"} TestClient {
       plaintext:=plaintext,
       encryptionContext:=encryptionContext,
       algorithmSuiteId:=None(),
-      materialsManager:=cmm);
+      materialsManager:=cmm,
+      frameLength:=Option.None(),
+      maxPlaintextLength:=Option.None());
     var res :- expect client.Encrypt(input);
 
     // Use Decrypt API
